store/client_proofs/create.v
@@ -7,7 +7,7 @@ From iris.heap_lang Require Import notation proofmode.
 From cryptis Require Import lib version term cryptis primitives tactics.
 From cryptis Require Import role session pk_auth pk_dh.
 From cryptis.store Require Import impl shared db.
-From cryptis.store.client_proofs Require Import store.
+From cryptis.store.client_proofs Require Import common.
 
 Set Implicit Arguments.
 Unset Strict Implicit.
@@ -29,5 +29,87 @@ Implicit Types γ : gname.
 Implicit Types v : val.
 
 Variable N : namespace.
+
+Lemma wp_client_create E c cs t1 t2 :
+  ↑cryptisN ⊆ E →
+  channel c -∗
+  store_ctx N -∗
+  public t1 -∗
+  public t2 -∗
+  {{{ client N cs }}}
+    Client.create N c (repr cs) t1 t2 @ E
+  {{{ (b : bool), RET #b;
+      client N cs ∗
+      if cst_ok cs && b then rem_mapsto cs t1 t2 else True }}}.
+Proof.
+iIntros "% #chan_c (_ & _ & _ & _ & _ & #? & #? & _)
+         #p_t1 #p_t2' !> %Φ client post".
+iDestruct "client" as "(%n & #handshake & #key & #minted & ts & client)".
+rewrite /Client.create. wp_pures.
+wp_bind (Client.get_timestamp _).
+iApply (wp_client_get_timestamp with "ts").
+iIntros "!> ts". wp_pures.
+wp_bind (Client.get_session_key _).
+iApply wp_client_get_session_key => //.
+iIntros "!> _". wp_pures.
+wp_list. wp_bind (tint _). iApply wp_tint. wp_list. wp_term_of_list. wp_pures.
+wp_tsenc. wp_pures.
+iMod (DB.create_client t2 _ _ t1 with "client")
+  as "(#create & client & up)".
+wp_bind (send _ _). iApply wp_send => //.
+{ iApply public_TEncIS => //.
+  - by rewrite minted_TKey.
+  - iModIntro. iExists (cst_name cs), n, t1, t2, (cst_ok cs).
+    by eauto 8.
+  - rewrite minted_of_list /= minted_TInt.
+    rewrite -[minted t1]public_minted -[minted t2]public_minted.
+    by eauto.
+  - iIntros "!> !> _".
+    rewrite public_of_list /= public_TInt. by eauto. }
+wp_pures.
+iCombine "post ts client up" as "I". iRevert "I".
+iApply wp_sess_recv => //.
+iIntros "!> %m (post & ts & client & up) #p_m". wp_pures.
+wp_list_of_term m; wp_pures; last by iLeft; iFrame.
+wp_list_match => [ts' k' v' b -> {m}|_] /=; wp_pures; last by iLeft; iFrame.
+wp_bind (tint _). iApply wp_tint.
+wp_eq_term e; wp_pures; last by iLeft; iFrame.
+subst ts'.
+wp_eq_term e; wp_pures; last by iLeft; iFrame.
+subst k'.
+wp_eq_term e; wp_pures; last by iLeft; iFrame.
+subst v'.
+wp_bind (Client.incr_timestamp _).
+iApply (wp_client_incr_timestamp with "ts").
+iIntros "!> ts".
+iDestruct (public_TEncE with "p_m [//]") as "{p_m} [[pub p_m]|p_m]".
+- wp_pures. wp_bind (tint _). iApply wp_tint. wp_pures.
+  case is_ok: cst_ok.
+  { iDestruct "key" as "[#contra _]".
+    iDestruct ("contra" with "pub") as ">[]". }
+  wp_bind (eq_term _ _). iApply wp_eq_term. wp_pures.
+  iModIntro. iRight. iExists _. iSplit => //.
+  iApply "post". iSplit => //.
+  iExists (S n). rewrite is_ok. iFrame. by eauto.
+- iDestruct "p_m" as "(#p_m & _)".
+  wp_pures. wp_bind (tint _). iApply wp_tint. wp_pures.
+  iDestruct "p_m" as "(%n' & %t1' & %t2' & %b' & %ok & %e &
+                       done' & free)".
+  case/Spec.of_list_inj: e => en <- _ ->.
+  have {en} <- : n = n' by lia.
+  wp_bind (eq_term _ _).
+  iApply (wp_wand _ _ _ (λ v, ⌜v = #b'⌝)%I).
+  { iApply wp_eq_term. iPureIntro. by case: b'. }
+  iIntros "% ->". wp_pures. iModIntro. iRight. iExists #b'.
+  iSplit => //. iApply "post".
+  iSplitL "client ts".
+  + iExists (S n). iFrame. by eauto.
+  + case is_ok: cst_ok => //=.
+    iPoseProof (handshake_done_agree with "key handshake done'") as "<-".
+    case: b' => //.
+    iDestruct "free" as "(%γ & key' & free)".
+    iPoseProof (wf_key_agree with "handshake key key'") as "<-".
+    by iApply "up".
+Qed.
 
 End Verif.
